haskell/aop/Cata.hs
@@ -1,0 +1,28 @@
+{-# LANGUAGE LambdaCase         #-}
+module  Cata
+    (   sum
+    ,   length
+    ,   average
+    )   where
+
+import Prelude  hiding (sum, length, div)
+import Data.Functor.Foldable
+import Data.Tuple.Extra
+
+(+++) :: b -> (a -> b -> b) -> ListF a b -> b
+(+++) b op = \case
+    Nil       -> b
+    Cons x y  -> op x y 
+
+div :: (Fractional a) => (a,Int) -> a
+div (a,n) = a / fromIntegral n
+
+sum :: (Num a) => [a] -> a
+sum = cata $  0 +++ (+)
+
+length :: [a] -> Int
+length = cata $ 0 +++ (\_ n -> n + 1)
+
+average :: (Fractional a) => [a] -> a
+average = div . (sum &&& length)
+
