lean/hhg/stmt.lean
@@ -3,19 +3,47 @@ def State : Type := string → ℕ
 def bind (x : string) (n : ℕ) (s:State) : State :=
   λ v, if v = x then n else s v
 
--- The WHILE language
+open list
+
+def env : list (string × ℕ) → State
+| []        := λ s, 0
+| ((v,n) :: xs) := λ s, if s = v then n else env xs s
+
+
+-- The WHILE language: deep embedding for actual language: full syntax and semantics specified
 inductive stmt : Type
 | skip    : stmt
-| assign  : string → (State → ℕ) → stmt
+| assign  : string → (State → ℕ) → stmt         -- shallow embedding for arithmetic expressions. Some function State → ℕ, not interested in syntax, semantics etc
 | seq     : stmt → stmt → stmt
-| ite     : (State → Prop) → stmt → stmt → stmt
+| ite     : (State → Prop) → stmt → stmt → stmt -- shallow embedding for boolean expressions. Actually using Prop rather than bool
 | while   : (State → Prop) → stmt → stmt
 
 infixr ` ;; ` : 90 := stmt.seq
 
+
 open stmt
 
+-- Big step semantics as a relation over State
 inductive BigStep : stmt → State → State → Prop
-| SKIP : ∀ (s:State), BigStep skip s s
-| ASN  : ∀ (x:string) (a:State → ℕ) (s:State), BigStep (assign x a) s (bind x (a s) s)
-| SEQ  : ∀ (e₁ e₂:stmt) (s t u:State), BigStep e₁ s t → BigStep e₂ t u → BigStep (e₁ ;; e₂) s u
+| SKIP    : ∀ (s:State), BigStep skip s s
+| ASN     : ∀ (x:string) (a:State → ℕ) (s:State), BigStep (assign x a) s (bind x (a s) s)
+| SEQ     : ∀ (e₁ e₂:stmt) (s u t:State), BigStep e₁ s u → BigStep e₂ u t → BigStep (e₁ ;; e₂) s t
+| IF_T    : ∀ (p:State → Prop) (e₁ e₂:stmt) (s t:State), p s → BigStep e₁ s t → BigStep (ite p e₁ e₂) s t
+| IF_F    : ∀ (p:State → Prop) (e₁ e₂:stmt) (s t:State), ¬(p s) → BigStep e₂ s t → BigStep (ite p e₁ e₂) s t
+| WHILE_T : ∀ (p:State → Prop) (e₁:stmt) (s u t:State), p s → BigStep e₁ s u → BigStep (while p e₁) u t → BigStep (while p e₁) s t
+| WHILE_F : ∀ (p:State → Prop) (e₁:stmt) (s:State), ¬(p s) → BigStep (while p e₁) s s
+
+def s0 : State := env [("x",3),("y",5)]
+def s1 : State := env [("x",8),("y",5)]
+def s2 : State := env [("x",8),("y",0)]
+
+def e1 : stmt := assign "x" (λ s, s "x" + s "y") ;; assign "y" (λ s, 0)
+
+open BigStep
+
+lemma L1 : BigStep e1 s0 s2 :=
+begin
+  apply (SEQ _ _ s0 s1 s2),
+    {apply (ASN "x" (λ s, s "x" + s "y") s0)},
+    {}
+end
