coq/set/Core/Replacement.v
@@ -10,8 +10,8 @@ Require Import Core.Functional.
 
 (* Axiom schema of replacement assuming LEM for our Coq meta-logic.             *)
 Theorem replacememtLEM : LEM -> forall (p:set -> set -> set -> Prop),
-    compatible3 p ->
-    forall (x:set), functional (p x) -> exists (y:set), forall (z:set),
+    compatible3 p    -> forall (x:set), 
+    functional (p x) -> exists (y:set), forall (z:set),
         z :: y <-> exists (u:set), u :: x /\ p x u z.
 Proof.
    intros L p C x F. 
